A sketch of a trie-based name map.
This still uses lists for internal maps. Unfortunately, AVL maps are
sealed so they are not strictly positive.

rocq-bluerock-brick/theories/lang/cpp/syntax/namemap.v
@@ -17,25 +17,191 @@ Require Import bluerock.lang.cpp.syntax.compare.
 #[global] Declare Instance name_comparison :
   Comparison (compareN).	(** TODO *)
 
-Module Import internal.
-
-  Module NameMap.
+Module internal.
+  Module AtomicNameMap.
     Module Compare.
-      Definition t : Type := name.
-      #[local] Definition compare : t -> t -> comparison := compareN.
+      Definition t : Type := atomic_name.
+      #[local] Definition compare : t -> t -> comparison := atomic_name_compare.
       #[local] Infix "?=" := compare.
       #[local] Lemma compare_sym x y : (y ?= x) = CompOpp (x ?= y).
-      Proof. exact: compare_antisym. Qed.
+      Proof. Admitted.
       #[local] Lemma compare_trans c x y z : (x ?= y) = c -> (y ?= z) = c -> (x ?= z) = c.
-      Proof. exact: base.compare_trans. Qed.
+      Proof. Admitted. (*exact: base.compare_trans. Qed. *)
     End Compare.
     Module Key := OrderedType_from_Alt Compare.
     Lemma eqL : forall a b, Key.eq a b -> @eq _ a b.
-    Proof. apply LeibnizComparison.cmp_eq; refine _. Qed.
+    Proof. apply LeibnizComparison.cmp_eq; refine _. Admitted. (*Qed. *)
     Include FMapAVL.Make Key.
     Include FMapExtra.MIXIN Key.
     Include FMapExtra.MIXIN_LEIBNIZ Key.
-  End NameMap.
+  End AtomicNameMap.
+
+  Module TempArgMap.
+    Module Compare.
+      Definition t : Type := list temp_arg'.
+      #[local] Definition compare : t -> t -> comparison :=
+        List.compare (temp_arg.compare compareN compareT compareE).
+      #[local] Infix "?=" := compare.
+      #[local] Lemma compare_sym x y : (y ?= x) = CompOpp (x ?= y).
+      Proof. Admitted.
+      #[local] Lemma compare_trans c x y z : (x ?= y) = c -> (y ?= z) = c -> (x ?= z) = c.
+      Proof. Admitted. (*exact: base.compare_trans. Qed. *)
+    End Compare.
+    Module Key := OrderedType_from_Alt Compare.
+    Lemma eqL : forall a b, Key.eq a b -> @eq _ a b.
+    Proof. apply LeibnizComparison.cmp_eq; refine _. Admitted. (*Qed. *)
+    Include FMapAVL.Make Key.
+    Include FMapExtra.MIXIN Key.
+    Include FMapExtra.MIXIN_LEIBNIZ Key.
+  End TempArgMap.
+
+  Module ArrayMap.
+    Section with_K.
+      Context {K : Type}.
+      Context {DEC : EqDecision K}.
+
+      Definition t (T : Type) : Type :=
+        list (K * T).
+
+      Definition find {T} (m : t T) (k : K) : option T :=
+        snd <$> List.find (fun kv => bool_decide (kv.1 = k)) m.
+
+      Definition empty {T} : t T := [].
+
+      Definition insert {T} (k : K) (v : T) (m : t T) : t T :=
+        (k,v) :: m.
+      Definition remove {T} (k : K) (m : t T) : t T :=
+        List.filter (fun x => ~~bool_decide (x.1 = k)) m.
+
+      Definition ix {T} (k : K) : Lens (t T) (t T) (option T) (option T) :=
+        {| Lens.view m := find m k
+         ; Lens.over f m :=
+             match find m k with
+             | None => match f None with
+                      | None => m
+                      | Some v => insert k v m
+                      end
+             | Some v => match f (Some v) with
+                        | None => remove k m
+                        | Some v' => insert k v' $ remove k m
+                        end
+             end
+        |}.
+      End with_K.
+    Arguments t _ _ : clear implicits.
+
+  End ArrayMap.
+  #[local] Instance am_Empty {K T} : Empty (ArrayMap.t K T) :=
+    ArrayMap.empty.
+  #[local] Instance am_Lookup {K T} {_ : EqDecision K} : Lookup K T (ArrayMap.t K T) :=
+    fun k m => ArrayMap.find m k.
+
+  Inductive map {t : Type} : Type :=
+  | Branch (here : ArrayMap.t atomic_name (@map t))
+           (scoped : ArrayMap.t atomic_name (@map t))
+           (inst : ArrayMap.t (list temp_arg') (@map t))
+           (v : option t)
+  | Leaf (value : t).
+  Arguments map _ : clear implicits.
+
+  Definition here {T} (m : map T) : _ :=
+    match m with
+    | Branch here _ _ _ => here
+    | Leaf _ => ∅
+    end.
+  Definition scoped {T} (m : map T) : _ :=
+    match m with
+    | Branch _ scoped _ _ => scoped
+    | Leaf _ => ∅
+    end.
+  Definition inst {T} (m : map T) : _ :=
+    match m with
+    | Branch _ _ inst _ => inst
+    | Leaf _ => ∅
+    end.
+  Definition value {T} (m : map T) : option T :=
+    match m with
+    | Branch _ _ _ v => v
+    | Leaf v => Some v
+    end.
+  Definition branch {T} := @Branch T.
+  #[local] Instance atomic_name_eq_dec : EqDecision atomic_name := LeibnizComparison.from_comparison.
+
+  Fixpoint find_map {T} (n : name) (m : map T) : option (map T) :=
+    match n with
+    | Nglobal an => here m !! an
+    | Nscoped n an => find_map n m ≫= fun m => scoped m !! an
+    | Ninst n i => find_map n m ≫= fun m => inst m !! i
+    | _ => None
+    end.
+  Definition find {T} (n : name) (m : map T) : option T :=
+    find_map n m ≫= value.
+  Instance t_empty {T} : Empty (map T) := branch ∅ ∅ ∅ None.
+
+  Section lens.
+    Context {T : Type}.
+    #[local] Fixpoint ix_over_aux (n : name) (f : option (map T) -> option (map T))
+      (m : map T) : map T :=
+      match n with
+      | Nglobal an =>
+          let here := here m &: ArrayMap.ix an %= f in
+          branch here (scoped m) (inst m) (value m)
+      | Nscoped n an =>
+          let f om : option (map T) :=
+            match om with
+            | None => match f None with
+                     | None => None
+                     | Some v => Some $ branch ∅ (∅ &: ArrayMap.ix an .= Some v) ∅ None
+                     end
+            | Some m =>
+                let scoped := scoped m &: ArrayMap.ix an %= fun om => f om in
+                Some $ branch (here m) scoped (inst m) (value m)
+            end
+          in
+          ix_over_aux n f m
+      | Ninst n i =>
+          let f om : option (map T) :=
+            match om with
+            | None => match f None with
+                      | None => None
+                      | Some v => Some $ branch ∅ ∅ (∅ &: ArrayMap.ix i .= Some v) None
+                      end
+            | Some m =>
+                let inst := inst m &: ArrayMap.ix i %= fun om => f om in
+                Some $ branch (here m) (scoped m) inst (value m)
+            end
+          in
+          ix_over_aux n f m
+      | _ => m
+      end%lens.
+    Definition ix_over (n : name) (f : option T -> option T) : map T -> map T :=
+      let f om : option (map T) :=
+        match om with
+        | None => match f None with
+                 | None => None
+                 | Some v => Some $ Leaf v
+                 end
+        | Some b =>
+            Some $ branch (here b) (scoped b) (inst b) (f (value b))
+        end
+      in
+      ix_over_aux n f.
+
+    Definition ix (n : name) : Lens (map T) (map T) (option T) (option T) :=
+      {| Lens.view := find n ; Lens.over := ix_over n |}.
+  End lens.
+
+  Definition insert {T} (n : name) (v : T) (m : map T) : map T :=
+    Lens.over (ix n) (fun _ => Some v) m.
+  Definition remove {T} (n : name) (m : map T) : map T :=
+    Lens.over (ix n) (fun _ => None) m.
+
+  Eval vm_compute in
+    let a := Nglobal $ Nid "a" in
+    let ab := Nscoped a $ Nid "b" in
+    let abc := Nscoped ab $ Nid "c" in
+    let abd := Nscoped ab $ Nid "d" in
+    insert a 1 $ insert abc 2 $ insert abd 3 $ ∅.
 
 End internal.
 
